code/experimental/P256/Hacl.Spec.P256.MontgomeryMultiplication.PointAdd.fst
@@ -336,7 +336,7 @@ let point_double_condition_seq u1 u2 s1 s2 z1 z2 =
     lemma_multiplication_not_mod_prime (felem_seq_as_nat z2) (modp_inv2 (pow2 256));
     lemmaFromDomain (felem_seq_as_nat z1);
     lemmaFromDomain (felem_seq_as_nat z2);
-    eq_u64 result (u64 0xffffffffffffffff)     
+  eq_u64 result (u64 0xffffffffffffffff)     
 
 
 inline_for_extraction noextract
